working on removing explicit indexing into lists

src/a_pre/Searching_and_splitting.thy
@@ -1,60 +1,53 @@
 theory Searching_and_splitting
-imports Key_value
+imports Key_value Disk_node Split_node
 begin
 
 (* Various definitions related to searching for a key in an ordered list of kv pairs, or a node
 frame *)
 
+(* construct an rsplit_node from a node and a search key *)
 
-(* insert and delete in list of kv ---------------------------------- *)
-
-(* insert a new kv into a list of kvs; used to insert new binding into a leaf *)
-primrec kvs_insert :: "'k ord \<Rightarrow> 'k*'v \<Rightarrow> ('k*'v)list \<Rightarrow> ('k*'v)list" where
-"kvs_insert cmp kv [] = [kv]"
-| "kvs_insert cmp kv (kv'#kvs') = (
-  let (k,v) = kv in
-  let (k',v') = kv' in
-  if key_lt cmp k' k then (k',v')#(kvs_insert cmp kv kvs')
-  else if (key_eq cmp k k') then (k,v)#kvs' else
-  (k,v)#(k',v')#kvs'
+(* NB ks_rs1 stored in reverse *)
+function aux' :: 
+  "'k ord \<Rightarrow> 'k \<Rightarrow> ('k list * 'a list) \<Rightarrow> ('k list * 'a list) \<Rightarrow> 
+    ('k list * 'a list) * 'a * ('k list * 'a list)" 
+where
+"aux' cmp k0 ks_rs1 ks_rs2 = (
+  let (ks1,rs1) = ks_rs1 in
+  let (ks,rs) = ks_rs2 in
+  let (r,rs') = (List.hd rs,List.tl rs) in
+  case ks of 
+  [] \<Rightarrow> ( (ks1,rs1), 
+          r, 
+          (ks,rs'))
+  | k#ks' \<Rightarrow> (
+    if key_lt cmp k0 k then
+      (* reached the right place *)
+      ( (ks1,rs1), 
+        r, 
+        (ks,rs'))
+    else 
+      aux' cmp k0  (k#ks1,r#rs1) (ks',rs'))
 )"
-
-definition kvs_insert_tests :: unit where
-"kvs_insert_tests = (
-  let _ = assert_true (kvs_insert nat_ord (2,2) (List.map (% x. (x,x)) [0,1,3,4]) = 
-    (List.map (% x. (x,x)) [0,1,2,3,4]))
-  in
-  let _ = assert_true (kvs_insert nat_ord (6,6) (List.map (% x. (x,x)) [0,1,3,4]) = 
-    (List.map (% x. (x,x)) [0,1,3,4,6]))
-  in
-  ())"
+apply (force)+ done
+termination aux'
+ by (force intro:FIXME)
 
 
-(* delete a pair with a particular key from a list of pairs *)
-definition kvs_delete :: "'k ord \<Rightarrow> 'k \<Rightarrow> ('k*'v)list \<Rightarrow> ('k*'v)list" where
-"kvs_delete ord k kvs = List.filter (% kv. ~ (key_eq ord (fst kv) k)) kvs"
-  
+definition mk_rsplit_node :: "'k ord \<Rightarrow> 'k \<Rightarrow> ('k list * 'r list) \<Rightarrow> ('k,'r)rsplit_node" where
+"
+mk_rsplit_node cmp k ks_rs = (
+  let ((ks1,rs1),r,(ks2,rs2)) = aux' cmp k ([],[]) ks_rs in
+  \<lparr>
+    r_ks1=ks1,
+    r_ts1=rs1,
+    r_t=r,
+    r_ks2=ks2,
+    r_ts2=rs2
+  \<rparr>)"
 
-(* search_key_to_index ---------------------------------------------- *)
+(* FIXME replace all the following with versions based on rsplit *)
 
-(* FIXME move *)
-
-(* return the index to the first key k1 st k < k1, or length of list if not found *)
-(*tr: assumes xs are sorted *)
-definition search_key_to_index :: "'k ord \<Rightarrow> 'k list => 'k => nat" where
-"search_key_to_index cmp ks k = (
-  let num_keys = length ks in
-  let i = List.find (% x. key_lt cmp k (ks!x)) (upt 0 num_keys) in
-  let i' = (case i of None => num_keys | Some x => x) in
-  let _ = check_true (% _. i' \<le> List.length ks) in
-  i')"
-
-definition sk2i_tests :: unit where
-"sk2i_tests = (
-  let sk2i = search_key_to_index nat_ord in
-  let _ = assert_true (sk2i [0,10,20,30,40] 20 = 3) in
-  let _ = assert_true (sk2i [0,10,20,30,40] 50 = 5) in
-  ())"
 
 
 (* split_ks_rs ------------------------------------------------------ *)
@@ -62,66 +55,22 @@ definition sk2i_tests :: unit where
 (* when splitting leaves and nodes, we need to split based on a
 particular key; also used when constructing frames *)
 
-(* this version is high level but slow; prefer following defn which
-TODO should be equivalent (!) *)
-
-(* given a key k and a list of (ks,rs), split and identify the child that 
-may contain k *)
-
-definition split_ks_rs' :: 
-  "'k ord \<Rightarrow> 'k \<Rightarrow> ('k list * 'a list) \<Rightarrow> ('k list * 'a list) * 'a * ('k list * 'a list)" where
-"split_ks_rs' cmp k ks_rs = (
-  let (ks,rs) = ks_rs in
-  let _ = check_true (% _. List.length rs = List.length ks + 1) in
-  let i = search_key_to_index cmp ks k in
-  let (ks1,ks2) = split_at i ks in
-  let (rs1,r',rs2) = split_at_3 i rs in
-  ((ks1,rs1),r',(ks2,rs2))
-)"
-  
-
-(* NB ks_rs1 stored in reverse *)
-function aux :: 
-  "'k ord \<Rightarrow> 'k \<Rightarrow> ('k list * 'a list) \<Rightarrow> ('k list * 'a list) \<Rightarrow> 
-    ('k list * 'a list) * 'a * ('k list * 'a list)" 
-where
-"aux cmp k0 ks_rs1 ks_rs2 = (
-  let (ks1,rs1) = ks_rs1 in
-  let (ks,rs) = ks_rs2 in
-  let (r,rs') = (List.hd rs,List.tl rs) in
-  case ks of 
-  [] \<Rightarrow> ( (List.rev ks1,List.rev rs1), 
-          r, 
-          (ks,rs'))
-  | k#ks' \<Rightarrow> (
-    if key_lt cmp k0 k then
-      (* reached the right place *)
-      ( (List.rev ks1,List.rev rs1), 
-        r, 
-        (ks,rs'))
-    else 
-      aux cmp k0  (k#ks1,r#rs1) (ks',rs'))
-)"
-apply (force)+ done
-termination aux
- by (force intro:FIXME)
-
-
-(* search through a list, and stop when we reach a position where
-k1\<le>k<k2, or equivalently (given ordered list) k < k2 *)
 
 definition split_ks_rs :: 
   "'k ord \<Rightarrow> 'k \<Rightarrow> ('k list * 'a list) \<Rightarrow> ('k list * 'a list) * 'a * ('k list * 'a list)" 
 where
 "split_ks_rs cmp k ks_rs = (
-  let res = aux cmp k ([],[]) ks_rs in
-(* FIXME forces generated code to have extra args; fixup in OCaml  let _ = check_true (% _. split_ks_rs' cmp k ks_rs = res) in *)
-  res)"
+  let r = mk_rsplit_node cmp k ks_rs in
+  let f = rsplit_to_split r in
+  (((f|>f_ks1),(f|>f_ts1)),(f|>f_t),((f|>f_ks2),(f|>f_ts2))))"
   
-(* NOTE tested via split_ks_rs' *)
+(* FIXME tested? *)
 
 
 (* insert aux funs: split_leaf and split_node ----------------------- *)
+
+(* FIXME these functions don't really belong here - they are a different kind
+of splitting, based on size not search key *)
 
 (* FIXME aren't these aux funs shared with its? *)
 
@@ -175,3 +124,90 @@ where
 
   
 end
+
+
+(* old ============================================================== *)
+
+
+
+(*
+(* search_key_to_index ---------------------------------------------- *)
+
+(* FIXME move *)
+
+(* return the index to the first key k1 st k < k1, or length of list if not found *)
+(*tr: assumes xs are sorted *)
+definition search_key_to_index :: "'k ord \<Rightarrow> 'k list => 'k => nat" where
+"search_key_to_index cmp ks k = (
+  let num_keys = length ks in
+  let i = List.find (% x. key_lt cmp k (ks!x)) (upt 0 num_keys) in
+  let i' = (case i of None => num_keys | Some x => x) in
+  let _ = check_true (% _. i' \<le> List.length ks) in
+  i')"
+
+definition sk2i_tests :: unit where
+"sk2i_tests = (
+  let sk2i = search_key_to_index nat_ord in
+  let _ = assert_true (sk2i [0,10,20,30,40] 20 = 3) in
+  let _ = assert_true (sk2i [0,10,20,30,40] 50 = 5) in
+  ())"
+*)
+
+
+
+
+(*
+
+(* this version is high level but slow; prefer following defn which
+TODO should be equivalent (!) *)
+
+(* given a key k and a list of (ks,rs), split and identify the child that 
+may contain k *)
+
+definition split_ks_rs' :: 
+  "'k ord \<Rightarrow> 'k \<Rightarrow> ('k list * 'a list) \<Rightarrow> ('k list * 'a list) * 'a * ('k list * 'a list)" where
+"split_ks_rs' cmp k ks_rs = (
+  let (ks,rs) = ks_rs in
+  let _ = check_true (% _. check_length_ks_rs (ks,rs)) in
+  let i = search_key_to_index cmp ks k in
+  let (ks1,ks2) = split_at i ks in
+  let (rs1,r',rs2) = split_at_3 i rs in
+  ((ks1,rs1),r',(ks2,rs2))
+)"
+  
+*)
+
+
+
+
+
+(*
+(* search through a list, and stop when we reach a position where
+k1\<le>k<k2, or equivalently (given ordered list) k < k2 *)
+
+(* NB ks_rs1 stored in reverse *)
+function aux :: 
+  "'k ord \<Rightarrow> 'k \<Rightarrow> ('k list * 'a list) \<Rightarrow> ('k list * 'a list) \<Rightarrow> 
+    ('k list * 'a list) * 'a * ('k list * 'a list)" 
+where
+"aux cmp k0 ks_rs1 ks_rs2 = (
+  let (ks1,rs1) = ks_rs1 in
+  let (ks,rs) = ks_rs2 in
+  let (r,rs') = (List.hd rs,List.tl rs) in
+  case ks of 
+  [] \<Rightarrow> ( (List.rev ks1,List.rev rs1), 
+          r, 
+          (ks,rs'))
+  | k#ks' \<Rightarrow> (
+    if key_lt cmp k0 k then
+      (* reached the right place *)
+      ( (List.rev ks1,List.rev rs1), 
+        r, 
+        (ks,rs'))
+    else 
+      aux cmp k0  (k#ks1,r#rs1) (ks',rs'))
+)"
+apply (force)+ done
+termination aux
+ by (force intro:FIXME)
+*)
